cedar-lean/Cedar/Thm/Data.lean
@@ -24,3 +24,4 @@ public import Cedar.Thm.Data.LT
 public import Cedar.Thm.Data.Map
 public import Cedar.Thm.Data.Set
 public import Cedar.Thm.Data.MapUnion
+public import Cedar.Thm.Data.String
